\documentclass[a4paper,twoside,12pt,hidelinks]{article}

% Packages
% ---------------------

\usepackage{amsmath} % Needed for command eqref
\usepackage{amsthm} % Used to show the proof box
\usepackage{fancyhdr} % Head and foot options
\usepackage{hyperref} % Uses automatic references \autoref
\usepackage[T1]{fontenc}
\usepackage{libertine}
\usepackage[libertine]{newtxmath} % Font

% Page settings
% ---------------------

\usepackage[top=2cm, bottom=2.5cm,left=2.5cm,right=2.5cm]{geometry} %  Page margins
\setlength{\parskip}{\baselineskip} % Add space between paragraphs
\setlength{\intextsep}{20pt plus 2.0pt minus 2.0pt} % Add vertical space before and after tables and figures (http://tex.stackexchange.com/a/26522/101976)
\parindent=0cm % Remove the paragraph indent of the first line
\addtolength{\jot}{2\jot} % Double the line between equations
\raggedbottom % Prevents spreading the page content vetically for non-full pages.

% Set vertical space around equations.
\AtBeginDocument{%
 \abovedisplayskip=15pt plus 5pt minus 5pt
 \abovedisplayshortskip=12pt plus 3pt
 \belowdisplayskip=15pt plus 5pt minus 5pt
 \belowdisplayshortskip=12pt plus 3pt minus 4pt
}


\begin{document}

\thispagestyle{empty}


\begin{align*}
  m_1 \ddot{\vec{r}}_1 & = \frac{G m_1 m_2}{r^3_{12}} \vec{r}_{12} + \frac{G m_1 m_3}{r^3_{13}} \vec{r}_{13} \\
  m_2 \ddot{\vec{r}}_2 & = - \frac{G m_1 m_2}{r^3_{12}} \vec{r}_{12} + \frac{G m_2 m_3}{r^3_{23}} \vec{r}_{23} \\
  m_3 \ddot{\vec{r}}_3 & = - \frac{G m_1 m_3}{r^3_{13}} \vec{r}_{13} - \frac{G m_2 m_3}{r^3_{23}} \vec{r}_{23}
\end{align*}

\[
  \vec{r}_{12} = \vec{r}_{2} - \vec{r}_{1}
\]

\[
  r_{12} = \sqrt{ (x_2 - x_1)^2 - (y_2 - y_1)^2 }
\]

\begin{align*}
  \ddot{x}_1 & = \frac{G m_2}{r^3_{12}} (x_2 - x_1)  + \frac{G m_3}{r^3_{13}} (x_3 - x_1) \\
  \ddot{y}_1 & = \frac{G m_2}{r^3_{12}} (y_2 - y_1)  + \frac{G m_3}{r^3_{13}} (y_3 - y_1) \\
  \ddot{x}_2 & = - \frac{G m_1}{r^3_{12}} (x_2 - x_1) + \frac{G m_3}{r^3_{23}} (x_3 - x_2) \\
  \ddot{y}_2 & = - \frac{G m_1}{r^3_{12}} (y_2 - y_1) + \frac{G m_3}{r^3_{23}} (y_3 - y_2) \\
  \ddot{x}_3 & = - \frac{G m_1 }{r^3_{13}} (x_3 - x_1) - \frac{G m_2}{r^3_{23}} (x_3 - x_2) \\
  \ddot{y}_3 & = - \frac{G m_1 }{r^3_{13}} (y_3 - y_1) - \frac{G m_2}{r^3_{23}} (y_3 - y_2)
\end{align*}



\begin{equation*}
  F = \frac{G m_1 m_2}{r^2}
\end{equation*}


\begin{equation*}
  \ddot{\vec{r}} = - \frac{G (m_1 + m_2)}{r^2} \hat{r}
\end{equation*}

\begin{equation*}
  \ddot{\vec{r}} = - \frac{1 + q}{r^2} \hat{r}
\end{equation*}

\begin{align*}
  \ddot{x} &= - \frac{1 + q}{r^3} x \\
  \ddot{y} &= - \frac{1 + q}{r^3} y
\end{align*}


\begin{align*}
  u_1 &= x \\
  u_2 &= y \\
  u_3 &= \dot{x} \\
  u_4 &= \dot{y}
\end{align*}


\begin{align*}
  \dot{u}_1 &= u_3 \\
  \dot{u}_2 &= u_4 \\
  \dot{u}_3 &= - \frac{1 + q}{r^3} u_1 \\
  \dot{u}_4 &= - \frac{1 + q}{r^3} u_2
\end{align*}


\end{document}